Updated md to include compilation info and cleaned up extraction code

src/extraction/AG_extraction_tweaks.hs
@@ -1,4 +1,6 @@
 -- In Preamble
+module AG_extracted_tweaked where
+
 import qualified Prelude
 import Prelude ((+), (*), fromInteger, signum, abs, negate)
 
