src/extraction/extracted/AG_example_operations.hs
@@ -1,0 +1,30 @@
+-- Example operations for extracted haskell code for algebraic graphs
+
+aG_vertices [1, 2, 3, 4]
+
+aG_edge 1 2
+
+aG_edges [(1, 2), (2, 3), (3, 4)]
+
+aG_makeGraph [1, 2, 3, 4] [(1, 2), (2, 3), (3, 4)]
+
+aG_transpose (1 + 2 * 3 + 1 * 5)
+
+aG_toList (1 + 2 * 3 + 1 * 5)
+
+aG_gmap (\x -> x + 1) (1 + 2 * 3 + 1 * 5)
+
+aG_mergeVertices (\x -> x Prelude.< 3) 30 (1 + 2 * 3 + 1 * 5)
+
+aG_bind (\x -> AG_vertex x + 30) (1 + 2 * 3 + 1 * 5)
+
+aG_induce (\x -> x Prelude.< 3) (1 + 2 * 3 + 1 * 5)
+
+aG_removeVertex 1 (1 + 2 * 3 + 1 * 5)
+
+aG_removeEdge 1 2 (1 * 2 + 2 * 1 + 1 * (2 + 3))
+
+aG_nodeAmount (1 + 2 * 3 + 1 * 5)
+
+aG_BFS [1] (1 + 2 * 3 + 1 * 5)
+
