src/extraction/extracted/IG_example_operations.hs
@@ -1,34 +1,4 @@
-aG_vertices [1, 2, 3, 4]
-
-aG_edge 1 2
-
-aG_edges [(1, 2), (2, 3), (3, 4)]
-
-aG_makeGraph [1, 2, 3, 4] [(1, 2), (2, 3), (3, 4)]
-
-aG_transpose (1 + 2 * 3 + 1 * 5)
-
-aG_toList (1 + 2 * 3 + 1 * 5)
-
-aG_gmap (\x -> x + 1) (1 + 2 * 3 + 1 * 5)
-
-aG_mergeVertices (\x -> x Prelude.< 3) 30 (1 + 2 * 3 + 1 * 5)
-
-aG_bind (\x -> AG_vertex x + 30) (1 + 2 * 3 + 1 * 5)
-
-aG_induce (\x -> x Prelude.< 3) (1 + 2 * 3 + 1 * 5)
-
-aG_removeVertex 1 (1 + 2 * 3 + 1 * 5)
-
-aG_removeEdge 1 2 (1 * 2 + 2 * 1 + 1 * (2 + 3))
-
-aG_nodeAmount (1 + 2 * 3 + 1 * 5)
-
-aG_BFS [1] (1 + 2 * 3 + 1 * 5)
-
-
-
-
+-- Example operations for extracted haskell code for inductive graphs
 
 iG_empty
 
